fine tuning

TaskinBA/CFG_To_PDA.thy
@@ -1,9 +1,9 @@
-section \<open>Equivalence of Context-Free Grammars and Pushdown Automata\<close>
+section \<open>Equivalence of CFG and PDA\<close>
 
-subsection \<open>Context-Free Grammars to Pushdown Automata\<close>
+subsection \<open>CFG to PDA\<close>
 
-text \<open>Given a context-free grammar, we construct a single-state pushdown automaton that only accepts words
-from the grammar's language. This formalization has been integrated from Leichtfried's Lean formalization\cite{lean}.\<close>
+text \<open>Starting from a CFG, we construct an equivalent single-state PDA.
+The formalization is based on the Lean formalization by Leichtfried\cite{lean}.\<close>
 
 theory CFG_To_PDA
   imports PDA Context_Free_Grammar.Context_Free_Grammar
@@ -32,23 +32,23 @@ locale cfg_to_pda =
   assumes finite_G: "finite (Prods G)"
 begin
 
-fun cfg_to_pda_trans_fun :: "sing_st \<Rightarrow> 't \<Rightarrow> ('n,'t) sym \<Rightarrow> (sing_st \<times> ('n,'t) syms) set" where
-  "cfg_to_pda_trans_fun Q_loop a (Tm b) = (if a = b then {(Q_loop, [])} else {})"
-| "cfg_to_pda_trans_fun _ _ _ = {}"
+fun pda_of_cfg :: "sing_st \<Rightarrow> 't \<Rightarrow> ('n,'t) sym \<Rightarrow> (sing_st \<times> ('n,'t) syms) set" where
+  "pda_of_cfg Q_loop a (Tm b) = (if a = b then {(Q_loop, [])} else {})"
+| "pda_of_cfg _ _ _ = {}"
 
-fun cfg_to_pda_eps_fun :: "sing_st \<Rightarrow> ('n,'t) sym \<Rightarrow> (sing_st \<times> ('n,'t) syms) set" where
-  "cfg_to_pda_eps_fun Q_loop (Nt A) = {(Q_loop, \<alpha>)| \<alpha>. (A, \<alpha>) \<in> Prods G}"
-| "cfg_to_pda_eps_fun _ _ = {}"
+fun pda_eps_of_cfg :: "sing_st \<Rightarrow> ('n,'t) sym \<Rightarrow> (sing_st \<times> ('n,'t) syms) set" where
+  "pda_eps_of_cfg Q_loop (Nt A) = {(Q_loop, \<alpha>)| \<alpha>. (A, \<alpha>) \<in> Prods G}"
+| "pda_eps_of_cfg _ _ = {}"
 
 definition cfg_to_pda_pda :: "(sing_st, 't, ('n,'t) sym) pda" where
   "cfg_to_pda_pda \<equiv> \<lparr> init_state = Q_loop, init_symbol = Nt (Start G), final_states = {}, 
-                    trans_fun = cfg_to_pda_trans_fun, eps_fun = cfg_to_pda_eps_fun \<rparr>"
+                    trans_fun = pda_of_cfg, eps_fun = pda_eps_of_cfg \<rparr>"
 
 lemma pda_cfg_to_pda: "pda cfg_to_pda_pda"
 proof (standard, goal_cases)
   case (1 p x z)
-  have "finite (cfg_to_pda_trans_fun p x z)"
-    by (induction p x z rule: cfg_to_pda_trans_fun.induct) auto
+  have "finite (pda_of_cfg p x z)"
+    by (induction p x z rule: pda_of_cfg.induct) auto
   then show ?case
     by (simp add: cfg_to_pda_pda_def)
 next
@@ -59,8 +59,8 @@ next
     by (simp add: finite_G)
   have "\<And>A. finite {(Q_loop, \<alpha>) |\<alpha>. (A, \<alpha>) \<in> Prods G}"
     using finite_subset[OF * **] by simp
-  hence "finite (cfg_to_pda_eps_fun p z)"
-    by (induction p z rule: cfg_to_pda_eps_fun.induct) auto
+  hence "finite (pda_eps_of_cfg p z)"
+    by (induction p z rule: pda_eps_of_cfg.induct) auto
   then show ?case
     by (simp add: cfg_to_pda_pda_def)
 qed
@@ -88,22 +88,22 @@ lemma cfg_to_pda_nt_cons:
   assumes "pda.step\<^sub>1 cfg_to_pda_pda (Q_loop, w, Nt A#\<gamma>) (Q_loop, w', \<beta>)"
   shows "\<exists>\<alpha>. (A, \<alpha>) \<in> Prods G \<and> \<beta> = \<alpha> @ \<gamma> \<and> w' = w"
 proof -
-  from assms have "(\<exists>\<beta>\<^sub>0. w' = w \<and> \<beta> = \<beta>\<^sub>0@\<gamma> \<and> (Q_loop, \<beta>\<^sub>0) \<in> cfg_to_pda_eps_fun Q_loop (Nt A)) 
-                     \<or> (\<exists>a \<beta>\<^sub>0. w = a # w' \<and> \<beta> = \<beta>\<^sub>0@\<gamma> \<and> (Q_loop,\<beta>\<^sub>0) \<in> cfg_to_pda_trans_fun Q_loop a (Nt A))"
+  from assms have "(\<exists>\<beta>\<^sub>0. w' = w \<and> \<beta> = \<beta>\<^sub>0@\<gamma> \<and> (Q_loop, \<beta>\<^sub>0) \<in> pda_eps_of_cfg Q_loop (Nt A)) 
+                     \<or> (\<exists>a \<beta>\<^sub>0. w = a # w' \<and> \<beta> = \<beta>\<^sub>0@\<gamma> \<and> (Q_loop,\<beta>\<^sub>0) \<in> pda_of_cfg Q_loop a (Nt A))"
     using pda.step\<^sub>1_rule[OF pda_cfg_to_pda] by (simp add: cfg_to_pda_pda_def)
   thus ?thesis
-    by (induction Q_loop "Nt A :: ('n, 't) sym" rule: cfg_to_pda_eps_fun.induct) auto
+    by (induction Q_loop "Nt A :: ('n, 't) sym" rule: pda_eps_of_cfg.induct) auto
 qed
 
 lemma cfg_to_pda_tm_stack_cons:
   assumes "pda.step\<^sub>1 cfg_to_pda_pda (Q_loop, w, Tm a # \<beta>) (Q_loop, w', \<beta>')"
   shows "w = a # w' \<and> \<beta> = \<beta>'"
 proof -
-  from assms have "(\<exists>\<beta>\<^sub>0. w' = w \<and> \<beta>' = \<beta>\<^sub>0@\<beta> \<and> (Q_loop, \<beta>\<^sub>0) \<in> cfg_to_pda_eps_fun Q_loop (Tm a)) 
-                   \<or> (\<exists>a\<^sub>0 \<beta>\<^sub>0. w = a\<^sub>0#w' \<and> \<beta>' = \<beta>\<^sub>0@\<beta> \<and> (Q_loop, \<beta>\<^sub>0) \<in> cfg_to_pda_trans_fun Q_loop a\<^sub>0 (Tm a))"
+  from assms have "(\<exists>\<beta>\<^sub>0. w' = w \<and> \<beta>' = \<beta>\<^sub>0@\<beta> \<and> (Q_loop, \<beta>\<^sub>0) \<in> pda_eps_of_cfg Q_loop (Tm a)) 
+                   \<or> (\<exists>a\<^sub>0 \<beta>\<^sub>0. w = a\<^sub>0#w' \<and> \<beta>' = \<beta>\<^sub>0@\<beta> \<and> (Q_loop, \<beta>\<^sub>0) \<in> pda_of_cfg Q_loop a\<^sub>0 (Tm a))"
     using pda.step\<^sub>1_rule[OF pda_cfg_to_pda] by (simp add: cfg_to_pda_pda_def)
   thus ?thesis
-    by (induction Q_loop "Tm a :: ('n, 't) sym" rule: cfg_to_pda_eps_fun.induct, auto) (metis emptyE, metis empty_iff prod.inject singletonD)
+    by (induction Q_loop "Tm a :: ('n, 't) sym" rule: pda_eps_of_cfg.induct, auto) (metis emptyE, metis empty_iff prod.inject singletonD)
 qed
 
 lemma cfg_to_pda_tm_stack_path:
@@ -115,11 +115,11 @@ proof -
     using pda.steps_not_refl_split_first[OF pda_cfg_to_pda] by blast
   have q'_def: "q' = Q_loop"
     using sing_st.exhaust by blast
-  from step1[unfolded q'_def] have "(\<exists>\<beta>\<^sub>0. w' = w \<and> \<alpha>' = \<beta>\<^sub>0@\<alpha> \<and> (Q_loop, \<beta>\<^sub>0) \<in> cfg_to_pda_eps_fun Q_loop (Tm a)) 
-                    \<or> (\<exists>a\<^sub>0 \<beta>\<^sub>0. w = a\<^sub>0#w' \<and> \<alpha>' = \<beta>\<^sub>0@\<alpha> \<and> (Q_loop, \<beta>\<^sub>0) \<in> cfg_to_pda_trans_fun Q_loop a\<^sub>0 (Tm a))"
+  from step1[unfolded q'_def] have "(\<exists>\<beta>\<^sub>0. w' = w \<and> \<alpha>' = \<beta>\<^sub>0@\<alpha> \<and> (Q_loop, \<beta>\<^sub>0) \<in> pda_eps_of_cfg Q_loop (Tm a)) 
+                    \<or> (\<exists>a\<^sub>0 \<beta>\<^sub>0. w = a\<^sub>0#w' \<and> \<alpha>' = \<beta>\<^sub>0@\<alpha> \<and> (Q_loop, \<beta>\<^sub>0) \<in> pda_of_cfg Q_loop a\<^sub>0 (Tm a))"
     using pda.step\<^sub>1_rule[OF pda_cfg_to_pda] by (simp add: cfg_to_pda_pda_def)
   hence "w = a # w' \<and> \<alpha>' = \<alpha>"
-    by (induction Q_loop "Tm a :: ('n, 't) sym" rule: cfg_to_pda_eps_fun.induct, auto) (metis empty_iff, metis empty_iff prod.inject singletonD)
+    by (induction Q_loop "Tm a :: ('n, 't) sym" rule: pda_eps_of_cfg.induct, auto) (metis empty_iff, metis empty_iff prod.inject singletonD)
   with steps q'_def show ?thesis by simp
 qed
 
@@ -157,7 +157,7 @@ lemma G_derives_if_cfg_to_pda_accepts:
   assumes "pda.steps cfg_to_pda_pda (Q_loop, w, \<alpha>) (Q_loop, [], [])"
   shows "Prods G \<turnstile> \<alpha> \<Rightarrow>* map Tm w"
 using assms proof (induction "(Q_loop, w, \<alpha>)" "(Q_loop, [] :: 't list, [] :: ('n, 't) syms)" 
-                      arbitrary: w \<alpha> rule: pda.steps_induct[OF pda_cfg_to_pda])
+                      arbitrary: w \<alpha> rule: pda.steps_induct2[OF pda_cfg_to_pda])
   case (3 w\<^sub>1 \<alpha>\<^sub>1 p\<^sub>2 w\<^sub>2 \<alpha>\<^sub>2)
   then show ?case proof (cases \<alpha>\<^sub>1)
     case (Cons Z' \<alpha>')
@@ -182,7 +182,7 @@ using assms proof (induction "(Q_loop, w, \<alpha>)" "(Q_loop, [] :: 't list, []
   qed (simp add: 3(1) pda.step\<^sub>1_empty_stack[OF pda_cfg_to_pda])
 qed (simp_all add: assms)
 
-lemma cfg_to_pda: "LangS G = pda.stack_accept cfg_to_pda_pda" (is "?L = ?P")
+lemma cfg_to_pda: "LangS G = pda.accept_stack cfg_to_pda_pda" (is "?L = ?P")
 proof
   show "?L \<subseteq> ?P"
   proof
@@ -195,7 +195,7 @@ proof
     hence "pda.steps cfg_to_pda_pda (Q_loop, x, [Nt (Start G)]) (Q_loop, [], [])"
       using cfg_to_pda_accepts_if_G_derives by simp
     thus "x \<in> ?P"
-      unfolding pda.stack_accept_def[OF pda_cfg_to_pda] by (auto simp: cfg_to_pda_pda_def)
+      unfolding pda.accept_stack_def[OF pda_cfg_to_pda] by (auto simp: cfg_to_pda_pda_def)
   qed
 next
   show "?P \<subseteq> ?L"
@@ -203,7 +203,7 @@ next
     fix x
     assume "x \<in> ?P"
     then obtain q where steps: "pda.steps cfg_to_pda_pda (Q_loop, x, [Nt (Start G)]) (q, [], [])"
-      unfolding pda.stack_accept_def[OF pda_cfg_to_pda] by (auto simp: cfg_to_pda_pda_def)
+      unfolding pda.accept_stack_def[OF pda_cfg_to_pda] by (auto simp: cfg_to_pda_pda_def)
     have "q = Q_loop"
       using sing_st.exhaust by blast
     with steps have "Prods G \<turnstile> [Nt (Start G)] \<Rightarrow>* map Tm x"
